revised FStar.HyperStack and FStar.HST to work with both eternal regions and stack regions that are ephemeral with push/pop; FStar.Buffer goes through, but needed to change the very last lemma in the file

ulib/FStar.HyperStack.fst
@@ -3,37 +3,97 @@ open FStar.HyperHeap
 module M  = FStar.Map
 module HH = FStar.HyperHeap
 
-inline let is_in (r:rid) (h:HH.t) = h `Map.contains` r
+let is_in (r:rid) (h:HH.t) = h `Map.contains` r
 
-assume val color: rid -> Tot int //TODO: enrich FStar.HyperHeap with this
 let is_stack_region r = color r > 0
 let is_eternal_region r  = color r <= 0
+
 type sid = r:rid{is_stack_region r} //stack region ids
-let is_above r1 r2 = r1 `includes` r2
-let is_just_below r1 r2 = r1 `extends` r2
-let is_below r1 r2 = r2 `is_above` r1
-assume Root_is_eternal: is_eternal_region HH.root
+
+let is_above r1 r2      = r1 `includes` r2
+let is_just_below r1 r2 = r1 `extends`  r2
+let is_below r1 r2      = r2 `is_above` r1
+let is_strictly_below r1 r2 = r1 `is_below` r2 && r1<>r2
+let is_strictly_above r1 r2 = r1 `is_above` r2 && r1<>r2
 
 let downward_closed (h:HH.t) = 
-  forall (r:rid). r=HH.root \/ (forall (s:rid). r `is_above` s ==> (is_stack_region r <==> is_stack_region s))
+  forall (r:rid). r `is_in` h  //for any region in the memory
+        ==> (r=HH.root    //either is the root
+	    \/ (forall (s:rid). r `is_above` s  //or, any region beneath it
+			  /\ s `is_in` h   //that is also in the memory
+		     ==> (is_stack_region r = is_stack_region s))) //must be of the same flavor as itself
 
-abstract let is_tip (tip:HH.rid) (h:HH.t) = 
+let is_tip (tip:HH.rid) (h:HH.t) = 
   (is_stack_region tip \/ tip=HH.root)                                  //the tip is a stack region, or the root
   /\ tip `is_in` h                                                      //the tip is active
-  /\ (forall (r:sid). r `is_in` h ==> r `is_above` tip)                      //any other sid activation is a parent of the tip
-  /\ (forall (r:rid). r `is_above` tip ==> r=HH.root \/ is_stack_region r)    //and every parent of tip is a stack region, except if it is the root
-  /\ (forall (r:rid{tip<>HH.root}). r `is_below` tip                                      //if tip is a stack region, then no region beyond the tip
-			     \/ (is_stack_region r /\ HH.disjoint r tip)             //             or any stack region disjoint from the tip
-		==> not (Map.contains h r))                            //is in the heap
+  /\ (forall (r:sid). r `is_in` h <==> r `is_above` tip)                      //any other sid activation is a above (or equal to) the tip
 
-noeq abstract type mem =
-  | HS : h:HH.t{HH.root `is_in` h /\ HH.map_invariant h /\ downward_closed h}        //the memory itself, always contains the root region, and the parent of any active region is active
+let hh = h:HH.t{HH.root `is_in` h /\ HH.map_invariant h /\ downward_closed h}        //the memory itself, always contains the root region, and the parent of any active region is active
+
+noeq type mem =
+  | HS : h:hh
        -> tip:rid{tip `is_tip` h}                                                   //the id of the current top-most region
        -> mem
+
+let empty_mem (m:HH.t) = 
+  let empty_map = Map.restrict (Set.empty) m in 
+  let h = Map.upd empty_map HH.root Heap.emp in 
+  let tip = HH.root in 
+  HS h tip
+ 
+let test0 (m:mem) (r:rid{r `is_above` m.tip}) = 
+    assert (r `is_in` m.h)
+
+let test1 (m:mem) (r:rid{r `is_above` m.tip}) = 
+    assert (r=HH.root \/ is_stack_region r)
+
+let test2 (m:mem) (r:sid{m.tip `is_above` r /\ m.tip <> r}) =  
+   assert (~ (r `is_in` m.h))
+
+let dc_elim (h:HH.t{downward_closed h}) (r:rid{r `is_in` h /\ r <> HH.root}) (s:rid)
+  : Lemma (r `is_above` s /\ s `is_in` h ==> is_stack_region r = is_stack_region s)
+  = ()	  
+
+let test3 (m:mem) (r:rid{r <> HH.root /\ is_eternal_region r /\ m.tip `is_above` r /\ is_stack_region m.tip})
+  : Lemma (~ (r `is_in` m.h))
+  = root_has_color_zero()
+
+let test4 (m:mem) (r:rid{r <> HH.root /\ is_eternal_region r /\ r `is_above` m.tip /\ is_stack_region m.tip})
+  : Lemma (~ (r `is_in` m.h))
+  = ()
+
+let eternal_region_does_not_overlap_with_tip (m:mem) (r:rid{is_eternal_region r /\ not (HH.disjoint r m.tip) /\ r<>HH.root /\ is_stack_region m.tip})
+  : Lemma (requires True)
+	  (ensures (~ (r `is_in` m.h)))
+  = root_has_color_zero()
+
+let poppable m = m.tip <> HH.root
+
+let remove_elt (#a:eqtype) (s:Set.set a) (x:a) = Set.intersect s (Set.complement (Set.singleton x))
+
+let popped m0 m1 =
+  poppable m0
+  /\ HH.parent m0.tip = m1.tip
+  /\ Set.equal (Map.domain m1.h) (remove_elt (Map.domain m0.h) m0.tip)
+  /\ Map.equal m1.h (Map.restrict (Map.domain m1.h) m0.h)
+
+let pop (m0:mem{poppable m0}) : GTot mem =
+  root_has_color_zero();
+  let dom = remove_elt (Map.domain m0.h) m0.tip in
+  let h0 = m0.h in
+  let h1 = Map.restrict dom m0.h in
+  let tip0 = m0.tip in
+  let tip1 = HH.parent tip0 in
+  assert (forall (r:sid). Map.contains h1 r ==>
+  	    (forall (s:sid). includes s r ==> Map.contains h1 s));
+  HS h1 tip1
 
 //A (reference a) may reside in the stack or heap
 noeq type reference (a:Type) =
   | MkRef : id:rid -> ref:HH.rref id a -> reference a
+
+let stackref (a:Type) = s:reference a { is_stack_region s.id }
+let ref (a:Type) = s:reference a{is_eternal_region s.id}
 
 let live_region (m:mem) (i:rid) =
   (is_eternal_region i \/ i `is_above` m.tip)
@@ -44,11 +104,11 @@ let contains (#a:Type) (m:mem) (s:reference a) =
   /\ HH.contains_ref s.ref m.h
 
 let upd (#a:Type) (m:mem) (s:reference a{live_region m s.id}) (v:a)
-  : Tot mem
+  : GTot mem
   = HS (m.h.[s.ref] <- v) m.tip
 
 let sel (#a:Type) (m:mem) (s:reference a)
-  : Tot a
+  : GTot a
   = m.h.[s.ref]
 
 let equal_domains (m0:mem) (m1:mem) =
@@ -69,27 +129,6 @@ let fresh_frame (m0:mem) (m1:mem) =
   /\ HH.parent m1.tip = m0.tip
   /\ m1.h == Map.upd m0.h m1.tip Heap.emp
 
-let poppable m = m.tip <> HH.root
-
-let remove_elt (#a:eqtype) (s:Set.set a) (x:a) = Set.intersect s (Set.complement (Set.singleton x))
-
-let popped m0 m1 =
-  poppable m0
-  /\ HH.parent m0.tip = m1.tip
-  /\ Set.equal (Map.domain m1.h) (remove_elt (Map.domain m0.h) m0.tip)
-  /\ Map.equal m1.h (Map.restrict (Map.domain m1.h) m0.h)
-
-let test (r:rid) (s:rid) = 
-  assert (r `is_below` s ==> s `is_above` r)
-  
-let pop (m0:mem{poppable m0}) : Tot mem =
-  let dom = remove_elt (Map.domain m0.h) m0.tip in
-  let h0 = m0.h in
-  let h1 = Map.restrict dom m0.h in
-  let tip0 = m0.tip in
-  let tip1 = HH.parent tip0 in
-  HS h1 tip1
-  
 let lemma_pop_is_popped (m0:mem{poppable m0})
   : Lemma (popped m0 (pop m0))
   = let m1 = pop m0 in
@@ -132,3 +171,8 @@ val lemma_live_1: #a:Type ->  #a':Type -> h:mem -> x:reference a -> x':reference
   (ensures  (x.id <> x'.id \/ ~ (as_ref x === as_ref x')))
   [SMTPat (contains h x); SMTPat (~(contains h x'))]
 let lemma_live_1 #a #a' h x x' = ()
+
+let above_tip_is_live (#a:Type) (m:mem) (x:reference a) : Lemma
+  (requires (x.id `is_above` m.tip))
+  (ensures (x.id `is_in` m.h))
+  = ()
